Earley/Proofs/Recognizer.lean
@@ -77,7 +77,7 @@ def earleyListSet (G : ContextFreeGrammarList T N) (w : List T) : Set (EarleyIte
 
 @[grind →]
 lemma binIdx_of_endIdx (G : ContextFreeGrammarList T N) (w : List T)
-    {bins : EarleyBins T N (w.length + 1)} (hbins : isWellFormedBins G w bins)
+    {bins : EarleyBins T N (w.length + 1)} (hbins : EarleyBins.WF G w bins)
     (x : EarleyItem T N) {k : Nat} (hk : k < w.length + 1)
     (hmem : x ∈ items bins[k]) : k = x.endIdx := by
   grind
@@ -90,45 +90,45 @@ lemma false_of_impossibleCompletedItem {G : ContextFreeGrammar T} [BEq G.NT] {x 
 
 section Subsets
 
-theorem updateBinAux_extensive (xs : List (BinItem T N)) (y : BinItem T N) :
+theorem updateBinAux_extensive (xs : BinItems T N) (y : BinItem T N) :
     items xs ⊆ items (updateBinAux y xs) := by
   induction xs generalizing y with
   | nil => grind
   | cons x xs ih => grind
 
-theorem updateBinAuxY_extensive (xs : List (BinItem T N)) (y : BinItem T N) :
+theorem updateBinAuxY_extensive (xs : BinItems T N) (y : BinItem T N) :
     y.item ∈ items (updateBinAux y xs) := by
   induction xs generalizing y with
   | nil => grind
   | cons x xs ih => grind
 
-theorem updateBin_extensive (xs ys : List (BinItem T N)) : items xs ⊆ items (updateBin xs ys) := by
+theorem updateBin_extensive (xs ys : BinItems T N) : items xs ⊆ items (updateBin xs ys) := by
   induction ys generalizing xs with
   | nil => grind
   | cons y ys ih => grind [updateBinAux_extensive]
 
-theorem updateBinY_extensive (xs ys : List (BinItem T N)) : items ys ⊆ items (updateBin xs ys) := by
+theorem updateBinY_extensive (xs ys : BinItems T N) : items ys ⊆ items (updateBin xs ys) := by
   induction ys generalizing xs with
   | nil => grind
   | cons y ys ih => grind [updateBinAuxY_extensive, updateBin_extensive]
 
 lemma updateBins_extensive {w : List T} {bins : EarleyBins T N (w.length + 1)}
-    (k i : Nat) (hi : i < w.length + 1) (newBin : List (BinItem T N)) :
+    (k i : Nat) (hi : i < w.length + 1) (newBin : BinItems T N) :
     items bins[i] ⊆ items (updateBins bins k newBin)[i] := by
   grind [updateBin_extensive]
 
 lemma updateBinsNewBin_extensive {w : List T} {bins : EarleyBins T N (w.length + 1)}
-    (k : Nat) (hk : k < w.length + 1) (newBin : List (BinItem T N)) :
+    (k : Nat) (hk : k < w.length + 1) (newBin : BinItems T N) :
     items newBin ⊆ items (updateBins bins k newBin)[k] := by
   grind [updateBinY_extensive]
 
 lemma setOfBinsUpdateBins_extensive {w : List T} {bins : EarleyBins T N (w.length + 1)}
-    (k : Nat) (newBin : List (BinItem T N)) :
+    (k : Nat) (newBin : BinItems T N) :
     setOfBins bins ⊆ setOfBins (updateBins bins k newBin) := by
   grind [updateBins_extensive]
 
 lemma earleyBinList_extensive {G : ContextFreeGrammarList T N} {w : List T}
-    {bins : EarleyBins T N (w.length + 1)} (hbins : isWellFormedBins G w bins)
+    {bins : EarleyBins T N (w.length + 1)} (hbins : EarleyBins.WF G w bins)
     (k j i : Nat) (hk : k < w.length + 1) (hi : i < w.length + 1) :
     items bins[i] ⊆ items (earleyBinList bins k hk j hbins).bins[i] := by
   fun_induction earleyBinList bins k hk j hbins with
@@ -136,7 +136,7 @@ lemma earleyBinList_extensive {G : ContextFreeGrammarList T N} {w : List T}
   | case2 bins hk j hbins hj x bins' hbins' => grind [updateBins_extensive]
 
 lemma lengthNth_le_lengthEarleyBinList {G : ContextFreeGrammarList T N} {w : List T}
-    {bins : EarleyBins T N (w.length + 1)} (hbins : isWellFormedBins G w bins)
+    {bins : EarleyBins T N (w.length + 1)} (hbins : EarleyBins.WF G w bins)
     (k j i : Nat) (hk : k < w.length + 1) (hi : i < w.length + 1) :
     bins[i].length ≤ (earleyBinList bins k hk j hbins).bins[i].length := by
   fun_induction earleyBinList bins k hk j hbins with
@@ -165,12 +165,12 @@ lemma lengthNth_le_lengthStepNth (Gₗ : ContextFreeGrammarList T N) {w : List T
   grind [lengthNth_le_lengthUpdateBinNth]
 
 lemma updateBins_idem_of_lower_idx {w : List T} {bins : EarleyBins T N (w.length + 1)}
-    (k i : Nat) (hk : k < w.length + 1) (hi : i < k) (newBin : List (BinItem T N)) :
+    (k i : Nat) (hk : k < w.length + 1) (hi : i < k) (newBin : BinItems T N) :
     (updateBins bins k newBin)[i] = bins[i] := by
   grind
 
 lemma earleyBinList_idem_of_lower_idx {G : ContextFreeGrammarList T N} {w : List T}
-    {bins : EarleyBins T N (w.length + 1)} (hbins : isWellFormedBins G w bins)
+    {bins : EarleyBins T N (w.length + 1)} (hbins : EarleyBins.WF G w bins)
     (k j n : Nat) (hk : k < w.length + 1) (hj : j < k) :
     (earleyBinList bins k hk n hbins).bins[j] = bins[j] := by
   fun_induction earleyBinList bins k hk n hbins with
@@ -179,7 +179,7 @@ lemma earleyBinList_idem_of_lower_idx {G : ContextFreeGrammarList T N} {w : List
 
 -- TODO: very notably, hj' is derivable from hj, but if I supply the proof on the fly via grind,
 --       the fun_induction isn't able to apply the cases correctly.
-lemma updateBinAux_getElem_of_lower_idx (xs : List (BinItem T N)) (y : BinItem T N) (j : Nat)
+lemma updateBinAux_getElem_of_lower_idx (xs : BinItems T N) (y : BinItem T N) (j : Nat)
     (hj : j < xs.length) (hj' : j < (updateBinAux y xs).length) :
     (updateBinAux y xs)[j].item = xs[j].item := by
   fun_induction updateBinAux y xs generalizing j with
@@ -189,7 +189,7 @@ lemma updateBinAux_getElem_of_lower_idx (xs : List (BinItem T N)) (y : BinItem T
   | case4 => grind
   | case5 => grind
 
-lemma updateBin_getElem_of_lower_idx (xs ys : List (BinItem T N)) (j : Nat) (hj : j < xs.length)
+lemma updateBin_getElem_of_lower_idx (xs ys : BinItems T N) (j : Nat) (hj : j < xs.length)
     (hj' : j < (updateBin xs ys).length) :
     ((updateBin xs ys)[j]'(by grind [length_le_lengthUpdateBin])).item = xs[j].item := by
   induction ys generalizing xs with
@@ -200,7 +200,7 @@ lemma updateBin_getElem_of_lower_idx (xs ys : List (BinItem T N)) (j : Nat) (hj 
     grind [updateBinAux_getElem_of_lower_idx]
 
 lemma updateBins_getElem_of_lower_idx {w : List T} {bins : EarleyBins T N (w.length + 1)}
-    (k j : Nat) (hk : k < w.length + 1) (hj : j < bins[k].length) (newBin : List (BinItem T N)) :
+    (k j : Nat) (hk : k < w.length + 1) (hj : j < bins[k].length) (newBin : BinItems T N) :
     ((updateBins bins k newBin)[k][j]'(by grind [lengthNth_le_lengthUpdateBinNth])).item
     = bins[k][j].item := by
   grind [updateBin_getElem_of_lower_idx]
@@ -208,7 +208,7 @@ lemma updateBins_getElem_of_lower_idx {w : List T} {bins : EarleyBins T N (w.len
 -- TODO: very notably, hlen is derivable from hj, but if I supply the proof on the fly via grind,
 --       the fun_induction isn't able to apply the cases correctly.
 lemma earleyBinList_getElem_of_lower_idx {G : ContextFreeGrammarList T N} {w : List T}
-    {bins : EarleyBins T N (w.length + 1)} (hbins : isWellFormedBins G w bins)
+    {bins : EarleyBins T N (w.length + 1)} (hbins : EarleyBins.WF G w bins)
     (k j i : Nat) (hk : k < w.length + 1) (hj : j < bins[k].length) (hij : j < i)
     (hlen : j < (earleyBinList bins k hk i hbins).bins[k].length) :
     (earleyBinList bins k hk i hbins).bins[k][j].item = bins[k][j].item := by
@@ -220,19 +220,19 @@ lemma earleyBinList_getElem_of_lower_idx {G : ContextFreeGrammarList T N} {w : L
     rw [ih]
     grind [updateBins_getElem_of_lower_idx]
 
-theorem updateBinAux_of_mem (xs : List (BinItem T N)) (y : BinItem T N) (hmem : y.item ∈ items xs) :
+theorem updateBinAux_of_mem (xs : BinItems T N) (y : BinItem T N) (hmem : y.item ∈ items xs) :
     items (updateBinAux y xs) = items xs := by
   induction xs generalizing y with
   | nil => grind
   | cons head tail ih => grind
 
-theorem updateBin_of_sub {xs : List (BinItem T N)} {ys : List (BinItem T N)}
-    (hmem : items ys ⊆ items xs) : items (updateBin xs ys) = items xs := by
+theorem updateBin_of_sub {xs : BinItems T N} {ys : BinItems T N} (hmem : items ys ⊆ items xs) :
+    items (updateBin xs ys) = items xs := by
   induction ys generalizing xs with
   | nil => grind
   | cons head tail ih => grind [updateBinAux_of_mem]
 
-theorem updateBins_of_sub {n k : Nat} {bins : EarleyBins T N n} {newBin : List (BinItem T N)}
+theorem updateBins_of_sub {n k : Nat} {bins : EarleyBins T N n} {newBin : BinItems T N}
     {hk : k < n} (hmem : items newBin ⊆ items bins[k]) :
     items (updateBins bins k newBin)[k] = items bins[k] := by
   grind [updateBin_of_sub]
@@ -244,13 +244,13 @@ theorem eqItems_of_completeList_of_eqItems {w : List T}
     items (completeList y bins1 hxS j) = items (completeList y bins2 hxS j) := by
   grind [completeList_eq_completeListI, completeListI]
 
-theorem eqItems_of_updateBinAux_of_eqEntry {xs : List (BinItem T N)} {y1 y2 : BinItem T N}
+theorem eqItems_of_updateBinAux_of_eqEntry {xs : BinItems T N} {y1 y2 : BinItem T N}
     (heqy : y1.item = y2.item) : items (updateBinAux y1 xs) = items (updateBinAux y2 xs) := by
   induction xs generalizing y1 y2 with
   | nil => grind
   | cons x xs ih => grind
 
-theorem eqItems_of_updateBinAux_of_eqBin {xs1 xs2 : List (BinItem T N)} {y : BinItem T N}
+theorem eqItems_of_updateBinAux_of_eqBin {xs1 xs2 : BinItems T N} {y : BinItem T N}
     (heqx : items xs1 = items xs2) : items (updateBinAux y xs1) = items (updateBinAux y xs2) := by
   induction xs1 generalizing y xs2 with
   | nil => grind
@@ -259,8 +259,8 @@ theorem eqItems_of_updateBinAux_of_eqBin {xs1 xs2 : List (BinItem T N)} {y : Bin
     · simp [items] at heqx
     · grind
 
-theorem eqItems_of_updateBin_of_eqBin {xs1 xs2 ys : List (BinItem T N)}
-    (heqx : items xs1 = items xs2) : items (updateBin xs1 ys) = items (updateBin xs2 ys) := by
+theorem eqItems_of_updateBin_of_eqBin {xs1 xs2 ys : BinItems T N} (heqx : items xs1 = items xs2) :
+    items (updateBin xs1 ys) = items (updateBin xs2 ys) := by
   induction ys generalizing xs1 xs2 with
   | nil => grind [List.map_eq_nil_iff]
   | cons y ys ih =>
@@ -270,7 +270,7 @@ theorem eqItems_of_updateBin_of_eqBin {xs1 xs2 ys : List (BinItem T N)}
     specialize ih hup
     apply ih
 
-theorem eqItems_of_updateBin_of_eqEntry (xs ys2 : List (BinItem T N)) {ys1 : List (BinItem T N)}
+theorem eqItems_of_updateBin_of_eqEntry (xs ys2 : BinItems T N) {ys1 : BinItems T N}
     (heqy : items ys1 = items ys2) :
     items (updateBin xs ys1) = items (updateBin xs ys2) := by
   induction ys1 generalizing ys2 xs with
@@ -287,7 +287,7 @@ theorem eqItems_of_updateBin_of_eqEntry (xs ys2 : List (BinItem T N)) {ys1 : Lis
       grind [eqItems_of_updateBin_of_eqBin]
 
 theorem eqItems_of_updateBins_of_eqItems {w : List T}
-    {bins1 bins2 : EarleyBins T N (w.length + 1)} {k : Nat} {newBin1 newBin2 : List (BinItem T N)}
+    {bins1 bins2 : EarleyBins T N (w.length + 1)} {k : Nat} {newBin1 newBin2 : BinItems T N}
     (heqB : ∀ n, ∀ (hn : n < w.length + 1), items bins1[n] = items bins2[n])
     (heqN : items newBin1 = items newBin2) :
     ∀ n, ∀ (hn : n < w.length + 1),
@@ -302,8 +302,8 @@ theorem eqItems_of_updateBins_of_eqItems {w : List T}
   grind
 
 theorem eqItems_of_earleyBinList_of_eqItems {G : ContextFreeGrammarList T N} {w : List T}
-    {bins1 bins2 : EarleyBins T N (w.length + 1)} (hbins1 : isWellFormedBins G w bins1)
-    (hbins2 : isWellFormedBins G w bins2) (k j : Nat) (hk : k < w.length + 1)
+    {bins1 bins2 : EarleyBins T N (w.length + 1)} (hbins1 : EarleyBins.WF G w bins1)
+    (hbins2 : EarleyBins.WF G w bins2) (k j : Nat) (hk : k < w.length + 1)
     (heq : ∀ n, ∀ (hn : n < w.length + 1), items bins1[n] = items bins2[n]) :
     ∀ n, ∀ (hn : n < w.length + 1),
     items (earleyBinList bins1 k hk j hbins1).bins[n] =
@@ -360,7 +360,7 @@ decreasing_by
   exact decreasingAux hbins1 j k hk (by lia)
 
 lemma setOfBinsEarleyBinList_extensive {G : ContextFreeGrammarList T N} {w : List T}
-    {bins : EarleyBins T N (w.length + 1)} (hbins : isWellFormedBins G w bins)
+    {bins : EarleyBins T N (w.length + 1)} (hbins : EarleyBins.WF G w bins)
     (k j : Nat) (hk : k < w.length + 1) :
     setOfBins bins ⊆ setOfBins (earleyBinList bins k hk j hbins).bins := by
   fun_induction earleyBinList bins k hk j hbins with
@@ -407,14 +407,14 @@ lemma earleyBinsList_extensive (G : ContextFreeGrammarList T N) (w : List T) (k 
 
 end Unused
 
-lemma updateBinAux_sub {s : Set (EarleyItem T N)} (xs : List (BinItem T N)) (y : BinItem T N)
+lemma updateBinAux_sub {s : Set (EarleyItem T N)} (xs : BinItems T N) (y : BinItem T N)
     (hx : {x | x ∈ items xs} ⊆ s) (hy : y.item ∈ s) :
     {z | z ∈ items (updateBinAux y xs) } ⊆ s := by
   induction xs generalizing y with
   | nil => grind
   | cons x xs ih => grind
 
-lemma updateBin_sub {s : Set (EarleyItem T N)} (xs ys : List (BinItem T N))
+lemma updateBin_sub {s : Set (EarleyItem T N)} (xs ys : BinItems T N)
     (hx : {x | x ∈ items xs} ⊆ s) (hy : {y | y ∈ items ys} ⊆ s) :
     {z | z ∈ items (updateBin xs ys) } ⊆ s := by
   induction ys generalizing xs with
@@ -423,7 +423,7 @@ lemma updateBin_sub {s : Set (EarleyItem T N)} (xs ys : List (BinItem T N))
 
 lemma updateBins_sub {w : List T} {bins : EarleyBins T N (w.length + 1)} {k : Nat}
     (hk : k < w.length + 1) {s : Set (EarleyItem T N)} (hb : setOfBins bins ⊆ s)
-    (newBin : List (BinItem T N)) (hn : {y | y ∈ items newBin} ⊆ s) :
+    (newBin : BinItems T N) (hn : {y | y ∈ items newBin} ⊆ s) :
     setOfBins (updateBins bins k newBin) ⊆ s := by
   intro z hmemz
   simp only [setOfBins, Order.lt_add_one_iff, Set.mem_setOf_eq] at hmemz
@@ -472,7 +472,7 @@ lemma initBins_sub_Model {G : ContextFreeGrammar T} [BEq G.NT] [LawfulBEq G.NT]
 
 lemma scanSet_sub_model {G : ContextFreeGrammar T} [BEq G.NT] [LawfulBEq G.NT]
     [LawfulBEq (EarleyItem T G.NT)] {w : List T} {Gₗ : ContextFreeGrammarList T G.NT}
-    {bins : EarleyBins T G.NT (w.length + 1)} (hbins : isWellFormedBins Gₗ w bins)
+    {bins : EarleyBins T G.NT (w.length + 1)} (hbins : EarleyBins.WF Gₗ w bins)
     (k j : Nat) (hk : k < w.length + 1) (hj : ¬j ≥ bins[k].length) (x : BinItem T G.NT)
     (hx : x = bins[k][j]) (t : T) (hsub : setOfBins bins ⊆ EarleySet G (mapT w))
     (hnext : x.item.nextSymbol = some (Symbol.terminal t)) (hw : ¬w.length ≤ k) :
@@ -490,7 +490,7 @@ lemma scanSet_sub_model {G : ContextFreeGrammar T} [BEq G.NT] [LawfulBEq G.NT]
 lemma predictSet_sub_model {G : ContextFreeGrammar T} [BEq G.NT] [LawfulBEq G.NT]
     [LawfulBEq (EarleyItem T G.NT)] {w : List T} {Gₗ : ContextFreeGrammarList T G.NT}
     (h : CFGEqCFGₗ G Gₗ) {bins : EarleyBins T G.NT (w.length + 1)}
-    (hbins : isWellFormedBins Gₗ w bins) (k j : Nat) (hk : k < w.length + 1)
+    (hbins : EarleyBins.WF Gₗ w bins) (k j : Nat) (hk : k < w.length + 1)
     (hj : ¬j ≥ bins[k].length) (x : BinItem T G.NT) (hx : x = bins[k][j]) (n : G.NT)
     (hsub : setOfBins bins ⊆ EarleySet G (mapT w))
     (hnext : x.item.nextSymbol = some (Symbol.nonterminal n)) :
@@ -511,7 +511,7 @@ lemma predictSet_sub_model {G : ContextFreeGrammar T} [BEq G.NT] [LawfulBEq G.NT
 
 lemma completeSet_sub_model {G : ContextFreeGrammar T} [BEq G.NT] [LawfulBEq G.NT]
     [LawfulBEq (EarleyItem T G.NT)] {w : List T} {Gₗ : ContextFreeGrammarList T G.NT}
-    {bins : EarleyBins T G.NT (w.length + 1)} (hbins : isWellFormedBins Gₗ w bins)
+    {bins : EarleyBins T G.NT (w.length + 1)} (hbins : EarleyBins.WF Gₗ w bins)
     (k j : Nat) (hk : k < w.length + 1) (hj : ¬j ≥ bins[k].length) (x : BinItem T G.NT)
     (hx : x = bins[k][j]) (hsub : setOfBins bins ⊆ EarleySet G (mapT w))
     (hnext : x.item.nextSymbol = none) :
@@ -549,7 +549,7 @@ lemma completeSet_sub_model {G : ContextFreeGrammar T} [BEq G.NT] [LawfulBEq G.N
 lemma earleyBinListSet_sub_model {G : ContextFreeGrammar T} [BEq G.NT] [LawfulBEq G.NT]
     [LawfulBEq (EarleyItem T G.NT)] (w : List T) {Gₗ : ContextFreeGrammarList T G.NT}
     (h : CFGEqCFGₗ G Gₗ) (bins : EarleyBins T G.NT (w.length + 1))
-    (hbins : isWellFormedBins Gₗ w bins) (hsub : setOfBins bins ⊆ EarleySet G (mapT w))
+    (hbins : EarleyBins.WF Gₗ w bins) (hsub : setOfBins bins ⊆ EarleySet G (mapT w))
     (k j : Nat) (hk : k < w.length + 1) :
     setOfBins (earleyBinList bins k hk j hbins).bins ⊆ EarleySet G (mapT w) := by
   fun_induction earleyBinList bins k hk j hbins with
@@ -578,7 +578,7 @@ lemma earleyBinListSet_sub_model {G : ContextFreeGrammar T} [BEq G.NT] [LawfulBE
 lemma earleyBinListZeroSet_sub_model {G : ContextFreeGrammar T} [BEq G.NT] [LawfulBEq G.NT]
     [LawfulBEq (EarleyItem T G.NT)] (w : List T) {Gₗ : ContextFreeGrammarList T G.NT}
     (h : CFGEqCFGₗ G Gₗ) (bins : EarleyBins T G.NT (w.length + 1))
-    (hbins : isWellFormedBins Gₗ w bins) (k : Nat) (hk : k < w.length + 1)
+    (hbins : EarleyBins.WF Gₗ w bins) (k : Nat) (hk : k < w.length + 1)
     (hsub : setOfBins bins ⊆ EarleySet G (mapT w)) :
     setOfBins (earleyBinList bins k hk 0 hbins).bins ⊆ EarleySet G (mapT w) := by
   grind [earleyBinListSet_sub_model]
@@ -641,7 +641,7 @@ section Completeness
 lemma completeList_idem {G : ContextFreeGrammar T} [BEq G.NT] [LawfulBEq G.NT]
     [LawfulBEq (EarleyItem T G.NT)] {w : List T} {Gₗ : ContextFreeGrammarList T G.NT}
     (heps : isEpsilonFree G) {bins bins' : EarleyBins T G.NT (w.length + 1)}
-    (hbins : isWellFormedBins Gₗ w bins) (hbins' : isWellFormedBins Gₗ w bins')
+    (hbins : EarleyBins.WF Gₗ w bins) (hbins' : EarleyBins.WF Gₗ w bins')
     (k j n : Nat) (hk : k < w.length + 1) (hj : ¬j ≥ bins[k].length) (hn : n < w.length + 1)
     (x : BinItem T G.NT) (hx : x = bins[k][j]) (hxS : x.item.startIdx < w.length + 1)
     (hnext : x.item.nextSymbol = none)
@@ -677,7 +677,7 @@ lemma completeList_idem {G : ContextFreeGrammar T} [BEq G.NT] [LawfulBEq G.NT]
 lemma earleyBinList_idem {G : ContextFreeGrammar T} [BEq G.NT] [LawfulBEq G.NT]
     [LawfulBEq (EarleyItem T G.NT)] {w : List T} {Gₗ : ContextFreeGrammarList T G.NT}
     (h : CFGEqCFGₗ G Gₗ) (heps : isEpsilonFree G)
-    {bins : EarleyBins T G.NT (w.length + 1)} (hbins : isWellFormedBins Gₗ w bins)
+    {bins : EarleyBins T G.NT (w.length + 1)} (hbins : EarleyBins.WF Gₗ w bins)
     (k j i n : Nat) (hk : k < w.length + 1) (hi : i ≤ j) (hn : n < w.length + 1)
     (hsub : setOfBins bins ⊆ EarleySet G (mapT w)) :
     items (earleyBinList bins k hk i hbins).bins[n] =
@@ -749,7 +749,7 @@ lemma earleyBinList_idem {G : ContextFreeGrammar T} [BEq G.NT] [LawfulBEq G.NT]
     match hnext : x.item.nextSymbol with
     | none =>
       simp only [hidem, hnext]
-      have inv1 : isWellFormedBins Gₗ w (updateBins
+      have inv1 : EarleyBins.WF Gₗ w (updateBins
           (earleyBinList bins' k hk (i + 1) hbins').bins k (completeList x.item
           (earleyBinList bins' k hk (i + 1) hbins').bins (by grind) j)) := by
         have heBL := (earleyBinList bins' k hk (i + 1) hbins').inv
@@ -768,7 +768,7 @@ lemma earleyBinList_idem {G : ContextFreeGrammar T} [BEq G.NT] [LawfulBEq G.NT]
           simp [hidem, hnext, hw]
         else
           simp only [hidem, hnext, hw, ↓reduceDIte]
-          have inv1 : isWellFormedBins Gₗ w (updateBins (earleyBinList bins' k hk (i + 1)
+          have inv1 : EarleyBins.WF Gₗ w (updateBins (earleyBinList bins' k hk (i + 1)
               hbins').bins (k+1) (scanList w x.item t k (by lia) j)) := by
             have heBL := (earleyBinList bins' k hk (i + 1) hbins').inv
             grind [wfBins_of_scanList]
@@ -789,7 +789,7 @@ lemma earleyBinList_idem {G : ContextFreeGrammar T} [BEq G.NT] [LawfulBEq G.NT]
             grind [updateBins_idem_of_lower_idx]
       | .nonterminal nt =>
         simp only [hidem, hnext]
-        have inv1 : isWellFormedBins Gₗ w (updateBins
+        have inv1 : EarleyBins.WF Gₗ w (updateBins
             (earleyBinList bins' k hk (i + 1) hbins').bins k (predictList Gₗ nt k)) := by
           have heBL := (earleyBinList bins' k hk (i + 1) hbins').inv
           grind [wfBins_of_predictList]
@@ -830,7 +830,7 @@ lemma initModel_sub_earleyBinListZero {G : ContextFreeGrammar T} [BEq G.NT] [Law
   apply @Set.mem_of_mem_of_subset _ ⟨r,0,0,0⟩ _ _ hsub this
 
 lemma scanMem_of_earleyBinListIndexAux {G : ContextFreeGrammarList T N} {w : List T}
-    {bins : EarleyBins T N (w.length + 1)} (hbins : isWellFormedBins G w bins)
+    {bins : EarleyBins T N (w.length + 1)} (hbins : EarleyBins.WF G w bins)
     (k j : Nat) (hk : k < w.length) (hj : ¬ (j ≥ bins[k].length))
     {x : EarleyItem T N} (hx : x = bins[k][j].item) (a : T)
     (hnext : bins[k][j].item.nextSymbol = some (Symbol.terminal a)) :
@@ -842,7 +842,7 @@ lemma scanMem_of_earleyBinListIndexAux {G : ContextFreeGrammarList T N} {w : Lis
   simp only [ge_iff_le, this, hj, ↓reduceDIte, hnext]
   have : y ∈ items (updateBins bins (k+1) (scanList w x a k (by lia) j))[k+1] := by
     grind [updateBinsNewBin_extensive]
-  have : isWellFormedBins G w
+  have : EarleyBins.WF G w
       (updateBins bins (k+1) (scanList w x a k (by lia) j)) := by
     grind [wfBins_of_scanList]
   have : y ∈ items (earleyBinList (updateBins bins (k+1) (scanList w x a k (by lia) j))
@@ -906,7 +906,7 @@ lemma scanModel_sub_scanL {G : ContextFreeGrammar T} [BEq G.NT] [LawfulBEq G.NT]
   apply Set.mem_of_mem_of_subset hmemT this (x := ⟨r, pos+1, i, k+1⟩)
 
 lemma predictMem_of_earleyBinListIndexAux {G : ContextFreeGrammarList T N} {w : List T}
-    {bins : EarleyBins T N (w.length + 1)} (hbins : isWellFormedBins G w bins)
+    {bins : EarleyBins T N (w.length + 1)} (hbins : EarleyBins.WF G w bins)
     (k j : Nat) (hk : k < w.length + 1) (hj : ¬ (j ≥ bins[k].length))
     (A : N) (hnext : bins[k][j].item.nextSymbol = some (Symbol.nonterminal A)) :
     items (predictList G A k) ⊆
@@ -916,7 +916,7 @@ lemma predictMem_of_earleyBinListIndexAux {G : ContextFreeGrammarList T N} {w : 
   simp only [ge_iff_le, hj, ↓reduceDIte, hnext]
   have : y ∈ items (updateBins bins k (predictList G A k))[k] := by
     grind [updateBinsNewBin_extensive]
-  have : isWellFormedBins G w (updateBins bins k (predictList G A k)) := by
+  have : EarleyBins.WF G w (updateBins bins k (predictList G A k)) := by
     grind [wfBins_of_predictList]
   have : y ∈ items (earleyBinList (updateBins bins k (predictList G A k)) k
     (by lia) (j + 1) this).bins[k] := by grind [earleyBinList_extensive]
@@ -925,7 +925,7 @@ lemma predictMem_of_earleyBinListIndexAux {G : ContextFreeGrammarList T N} {w : 
 lemma predictMem_of_earleyBinListIndex {G : ContextFreeGrammar T} [BEq G.NT] [LawfulBEq G.NT]
     [LawfulBEq (EarleyItem T G.NT)] {w : List T} {Gₗ : ContextFreeGrammarList T G.NT}
     (h : CFGEqCFGₗ G Gₗ) (heps : isEpsilonFree G) {bins : EarleyBins T G.NT (w.length + 1)}
-    (hbins : isWellFormedBins Gₗ w bins) (k j : Nat) (hk : k < w.length + 1)
+    (hbins : EarleyBins.WF Gₗ w bins) (k j : Nat) (hk : k < w.length + 1)
     (hj : ¬ (j ≥ (earleyBinList bins k (by lia) 0 hbins).bins[k].length)) (A : G.NT)
     (hnext : (earleyBinList bins k (by lia) 0 hbins).bins[k][j].item.nextSymbol
       = some (Symbol.nonterminal A)) (hSound : setOfBins bins ⊆ EarleySet G (mapT w)) :
@@ -942,7 +942,7 @@ lemma predictMem_of_earleyBinListIndex {G : ContextFreeGrammar T} [BEq G.NT] [La
 lemma predictModel_sub_predictL {G : ContextFreeGrammar T} [BEq G.NT] [LawfulBEq G.NT]
     [LawfulBEq (EarleyItem T G.NT)] {w : List T} {Gₗ : ContextFreeGrammarList T G.NT}
     (h : CFGEqCFGₗ G Gₗ) (heps : isEpsilonFree G) {bins : EarleyBins T G.NT (w.length + 1)}
-    (hbins : isWellFormedBins Gₗ w bins) {k : Nat} {r2 : ContextFreeRule T G.NT}
+    (hbins : EarleyBins.WF Gₗ w bins) {k : Nat} {r2 : ContextFreeRule T G.NT}
     {x : EarleyItem T G.NT} (hk : k < w.length + 1)
     (ih : x ∈ items (earleyBinList bins k (by lia) 0 hbins).bins[k]) (hmemr2 : r2 ∈ Gₗ.rules)
     (hnext : x.nextSymbol = some (Symbol.nonterminal r2.input))
@@ -963,7 +963,7 @@ lemma predictModel_sub_predictL {G : ContextFreeGrammar T} [BEq G.NT] [LawfulBEq
   apply Set.mem_of_mem_of_subset hmemT this (x := ⟨r2, 0, k, k⟩)
 
 lemma completeMem_of_earleyBinListIndexAux {G : ContextFreeGrammarList T N} {w : List T}
-    {bins : EarleyBins T N (w.length + 1)} (hbins : isWellFormedBins G w bins)
+    {bins : EarleyBins T N (w.length + 1)} (hbins : EarleyBins.WF G w bins)
     {posy j k n : Nat} {r2 : ContextFreeRule T N} {y : EarleyItem T N}
     (hk : k < w.length + 1) (hj : j < w.length + 1) (hn : ¬ (n ≥ bins[k].length))
     (hy : y = ⟨r2, posy, j, k⟩) (hmemy : y = bins[k][n].item)
@@ -977,7 +977,7 @@ lemma completeMem_of_earleyBinListIndexAux {G : ContextFreeGrammarList T N} {w :
   have hyS : y.startIdx < w.length + 1 := by grind
   have : z ∈ items (updateBins bins k (completeList y bins hyS n))[k] := by
     grind [updateBinsNewBin_extensive]
-  have : isWellFormedBins G w (updateBins bins k (completeList y bins hyS n)) := by
+  have : EarleyBins.WF G w (updateBins bins k (completeList y bins hyS n)) := by
     grind [wfBins_of_completeList]
   have : z ∈ items (earleyBinList (updateBins bins k (completeList y bins hyS n)) k
       (by lia) (n + 1) this).bins[k] := by
@@ -987,7 +987,7 @@ lemma completeMem_of_earleyBinListIndexAux {G : ContextFreeGrammarList T N} {w :
 lemma completeMem_of_earleyBinListIndex {G : ContextFreeGrammar T} [BEq G.NT] [LawfulBEq G.NT]
     [LawfulBEq (EarleyItem T G.NT)] {w : List T} {Gₗ : ContextFreeGrammarList T G.NT}
     (h : CFGEqCFGₗ G Gₗ) (heps : isEpsilonFree G) {bins : EarleyBins T G.NT (w.length + 1)}
-    (hbins : isWellFormedBins Gₗ w bins) {posy j k n : Nat} {r2 : ContextFreeRule T G.NT}
+    (hbins : EarleyBins.WF Gₗ w bins) {posy j k n : Nat} {r2 : ContextFreeRule T G.NT}
     {y : EarleyItem T G.NT} (hk : k < w.length + 1) (hj : j < w.length + 1)
     (hn : ¬ (n ≥ (earleyBinList bins k (by lia) 0 hbins).bins[k].length))
     (hy : y = ⟨r2, posy, j, k⟩)
@@ -1005,7 +1005,7 @@ lemma completeMem_of_earleyBinListIndex {G : ContextFreeGrammar T} [BEq G.NT] [L
 lemma completeModel_sub_completeL {G : ContextFreeGrammar T} [BEq G.NT] [LawfulBEq G.NT]
     [LawfulBEq (EarleyItem T G.NT)] {w : List T} {Gₗ : ContextFreeGrammarList T G.NT}
     (h : CFGEqCFGₗ G Gₗ) (heps : isEpsilonFree G) {bins : EarleyBins T G.NT (w.length + 1)}
-    (hbins : isWellFormedBins Gₗ w bins) {posx posy i j k : Nat} {r1 r2 : ContextFreeRule T G.NT}
+    (hbins : EarleyBins.WF Gₗ w bins) {posx posy i j k : Nat} {r1 r2 : ContextFreeRule T G.NT}
     {x y : EarleyItem T G.NT} (hk : k < w.length + 1) (hj : j < w.length + 1)
     (hx : x = ⟨r1, posx, i, j⟩) (hy : y = ⟨r2, posy, j, k⟩)
     (hmemxL : x ∈ items (earleyBinList bins k (by lia) 0 hbins).bins[j])
